Factor out trace properties from actor properties

theories/ToySep.v
@@ -22,8 +22,7 @@ Import ListNotations.
 Reserved Notation "aid '@' req '<~' ret" (at level 30).
 
 Section IOHandler.
-  Variable AID : Set.
-  Context {AID_ord : OrderedType AID}.
+  Context {AID : Set} `{AID_ord : OrderedType AID}.
 
   Inductive HandlerRet {req_t state_t : Type} (req : req_t) (rep_t : req_t -> Set) : Type :=
   | r_return : forall (reply : rep_t req)
@@ -35,7 +34,7 @@ Section IOHandler.
 
   Record t : Type :=
     {
-      h_state         : Type;
+      h_state         : Set;
       h_req           : Set;
       h_ret           : h_req -> Set;
       h_initial_state : Nondeterministic h_state;
@@ -44,200 +43,215 @@ Section IOHandler.
                           (req : h_req),
                         Nondeterministic @HandlerRet h_req h_state req h_ret;
     }.
-
-  Section Actor.
-    Variable H : t.
-
-    CoInductive Actor : Type :=
-    | a_cont : forall (pending_req : H.(h_req))
-                 (continuation : H.(h_ret) pending_req -> option Actor)
-             , Actor.
-
-    Definition Actors := Map[AID, Actor].
-
-    Record TraceElem : Set :=
-      trace_elem { te_aid : AID;
-                   te_req : H.(h_req);
-                   te_ret : H.(h_ret) te_req;
-                 }.
-
-    Definition Trace := list TraceElem.
-
-    Record ModelState : Type :=
-      mkState
-        {
-          m_actors : Actors;
-          m_state  : H.(h_state);
-        }.
-
-    Definition enter_syscall aid (req : h_req H) cont (ret : HandlerRet req (h_ret H)) ms :=
-      match ms with
-        {| m_state := s; m_actors := aa |} =>
-        match ret with
-        | r_stall _ _         => ms
-        | r_return _ _ rep s' =>
-          let aa' := match cont rep with
-                     | Some a' => add aid a' aa
-                     | None    => remove aid aa
-                     end in
-          mkState aa' s'
-        end
-      end.
-
-    Definition is_reachable (ms ms' : ModelState) (aid : AID) (HIn : In aid (m_actors ms)) : Prop :=
-      match ms with
-        {| m_state := s |} =>
-        match find' aid (m_actors ms) HIn with
-        | a_cont req cont =>
-          exists ret : @HandlerRet H.(h_req) H.(h_state) req H.(h_ret),
-            H.(h_eval) s aid req ret /\
-            ms' = enter_syscall aid req cont ret ms
-        end
-      end.
-
-    (** Constructively define a property that certain model state is
-    reachable from a given deterministic program [initial_actors] and
-    nondeterministic handler state *)
-    Inductive ReachableState {initial_actors : Actors} : ModelState -> Prop :=
-    | model_init : forall s0,
-        H.(h_initial_state) s0 ->
-        ReachableState {| m_actors := initial_actors;
-                          m_state  := s0;
-                       |}
-
-    | model_step : forall (aid : AID) (ms ms' : ModelState) (HIn : In aid (m_actors ms)),
-        is_reachable ms ms' aid HIn ->
-        ReachableState ms ->
-        ReachableState ms'.
-
-    (** Note: The following definition is completely related to the
-    IOHandler and doesn't assume anything about the actors'
-    behavior. Therefore it can be used to define undesirable trace
-    sequences. *)
-    Definition valid_trace_elem (ms : ModelState) (te : TraceElem) (s' : H.(h_state)) : Prop :=
-      match te, ms with
-      | trace_elem aid req ret, mkState _ s =>
-        let hret := r_return req (h_ret H) ret s' in
-        h_eval H s aid req hret
-      end.
-
-    Transparent valid_trace_elem.
-
-    (** The following definition very much depend on the actors'
-    behavior! It can be used together with actor invariants to prove
-    that undesirable traces are impossible under actor definition. *)
-    Definition valid_transition (ms : ModelState) (te : TraceElem) (s' : H.(h_state)) :=
-       match te, ms with
-       | trace_elem aid req ret, mkState aa s =>
-         {HIn : In aid aa |
-          let HReq := match find' aid aa HIn with
-                      | a_cont req' _ => req = req'
-                      end in
-          HReq /\ valid_trace_elem ms te s'}
-       end.
-
-    Definition apply_trace_elem (ms : ModelState) (te : TraceElem) (s' : H.(h_state))
-               (Hte : valid_transition ms te s') : ModelState.
-      destruct te as [aid req ret].
-      destruct ms as [aa s].
-      destruct Hte as [HIn [Hreq Hs]].
-      destruct (find' aid aa HIn) as [req0 cont].
-      refine (enter_syscall aid req0 cont _ (mkState aa s)).
-      - rewrite <-Hreq.
-        apply (r_return _ _ ret s').
-    Defined.
-
-    Lemma apply_trace_elem_reachable : forall {initial_actors} (ms : ModelState) (te : TraceElem) s',
-        @ReachableState initial_actors ms ->
-        forall Hte : valid_transition ms te s',
-          @ReachableState initial_actors (apply_trace_elem ms te s' Hte).
-    Proof.
-      intros initial_actors ms te s' Hms Hte.
-      unfold valid_transition in Hte.
-      unfold valid_trace_elem in Hte.
-      destruct te as [aid req ret].
-      destruct ms as [aa s].
-      destruct Hte as [HIn [Hreq Heval]].
-      refine (model_step aid (mkState aa s) _ HIn _ Hms).
-      simpl.
-      destruct (find' aid aa HIn) as [req' cont].
-      destruct Hreq.
-      exists (r_return _ _ ret s').
-      easy.
-    Qed.
-  End Actor.
-
-  Section ComposeHandlers.
-    Definition compose_state h1 h2 : Type :=
-      h_state h1 * h_state h2.
-
-    Definition compose_req h1 h2 : Set :=
-      h_req h1 + h_req h2.
-
-    Hint Transparent compose_state.
-
-    Definition compose_initial_state h1 h2 state :=
-      h1.(h_initial_state) (fst state) /\ h2.(h_initial_state) (snd state).
-
-    Hint Transparent compose_initial_state.
-
-    Definition compose_ret_t (h1 h2 : t) (req : compose_req h1 h2) : Set :=
-      match req with
-      | inl l => h1.(h_ret) l
-      | inr r => h2.(h_ret) r
-      end.
-
-    Hint Transparent compose_ret_t.
-
-    Definition ComposeHandlerRet h1 h2 req : Type :=
-      @HandlerRet (compose_req h1 h2)
-                  (compose_state h1 h2)
-                  req
-                  (compose_ret_t h1 h2).
-
-    Definition compose_eval h1 h2
-               (state : compose_state h1 h2)
-               (aid : AID)
-               req
-               (ret : ComposeHandlerRet h1 h2 req) : Prop.
-      refine (
-          (let (s1, s2) := state in
-           match req as req' return (req = req' -> Prop) with
-           | inl req' => fun H => h1.(h_eval) s1 aid req' _
-           | inr req' => fun H => h2.(h_eval) s2 aid req' _
-           end) (eq_refl req));
-        subst;
-        destruct ret;
-        try simpl in reply;
-        constructor; assumption.
-    Defined.
-
-    Definition compose (h1 h2 : t) : t :=
-      {| h_state         := compose_state h1 h2;
-         h_req           := compose_req h1 h2;
-         h_ret           := compose_ret_t h1 h2;
-         h_initial_state := compose_initial_state h1 h2;
-         h_eval          := compose_eval h1 h2;
-      |}.
-  End ComposeHandlers.
 End IOHandler.
 
-Notation "aid '@' req '<~' ret" := (trace_elem aid req ret).
+Section Trace.
+  Variable AID : Set.
+  Variable H : @t AID.
 
-Arguments compose {_}.
-Arguments h_state {_}.
-Arguments h_req {_}.
-Arguments h_ret {_}.
-Arguments h_initial_state {_}.
-Arguments h_eval {_}.
-Arguments Actor {_} {_}.
-Arguments a_cont {_} {_}.
-Arguments ModelState {_} {_}.
-Arguments m_actors {_} {_} {_}.
-Arguments m_state {_} {_} {_}.
-Arguments ReachableState {_} {_}.
-Arguments model_init {_} {_} {_} {_}.
-Arguments model_step {_} {_} {_} {_}.
+  Record TraceElem : Set :=
+    trace_elem { te_aid : AID;
+                 te_req : H.(h_req);
+                 te_ret : H.(h_ret) te_req;
+               }.
+
+  Definition Trace := list TraceElem.
+
+  Definition valid_trace_elem (te : TraceElem) (s s' : H.(h_state)) : Prop :=
+    match te with
+    | trace_elem aid req ret =>
+      let hret := r_return req (h_ret H) ret s' in
+      h_eval H s aid req hret
+    end.
+
+  (** Property that tells if a certain sequence of side effects is
+  "physically possible". E.g. mutex can't be taken twice, messages
+  don't travel backwards in time, memory doesn't change all by
+  itself and so on: *)
+  Inductive PossibleTrace (state : H.(h_state)) : Trace -> Prop :=
+  | pt_nil : PossibleTrace state []
+
+  | pt_cons : forall (state' : H.(h_state)) (trace_elem : TraceElem) (trace_tail : Trace),
+        valid_trace_elem trace_elem state state' ->
+        PossibleTrace state' trace_tail ->
+        PossibleTrace state (trace_elem :: trace_tail).
+End Trace.
+
+Global Arguments TraceElem {_} {_}.
+Global Arguments te_aid {_} {_}.
+Global Arguments te_req {_} {_}.
+Global Arguments te_ret {_} {_}.
+Global Arguments trace_elem {_} {_}.
+Global Arguments PossibleTrace {_} {_}.
+Global Arguments pt_nil {_} {_}.
+Global Arguments pt_cons {_} {_}.
+Global Arguments valid_trace_elem {_} {_}.
+
+Section Actor.
+  Context {AID : Set} `{AID_ord : OrderedType AID} {H : @t AID}.
+
+  CoInductive Actor : Type :=
+  | a_cont : forall (pending_req : H.(h_req))
+               (continuation : H.(h_ret) pending_req -> option Actor)
+           , Actor.
+
+  Definition Actors := Map[AID, Actor].
+
+  Record ModelState : Type :=
+    mkState
+      {
+        m_actors : Actors;
+        m_state  : H.(h_state);
+      }.
+
+  Definition enter_syscall aid (req : h_req H) cont (ret : HandlerRet req (h_ret H)) ms :=
+    match ms with
+      {| m_state := s; m_actors := aa |} =>
+      match ret with
+      | r_stall _ _         => ms
+      | r_return _ _ rep s' =>
+        let aa' := match cont rep with
+                   | Some a' => add aid a' aa
+                   | None    => remove aid aa
+                   end in
+        mkState aa' s'
+      end
+    end.
+
+  Definition is_reachable (ms ms' : ModelState) (aid : AID) (HIn : In aid (m_actors ms)) : Prop :=
+    match ms with
+      {| m_state := s |} =>
+      match find' aid (m_actors ms) HIn with
+      | a_cont req cont =>
+        exists ret : @HandlerRet H.(h_req) H.(h_state) req H.(h_ret),
+          H.(h_eval) s aid req ret /\
+          ms' = enter_syscall aid req cont ret ms
+      end
+    end.
+
+  (** Constructively define a property that certain model state is
+  reachable from a given deterministic program [initial_actors] and
+  nondeterministic handler state *)
+  Inductive ReachableState {initial_actors : Actors} : ModelState -> Prop :=
+  | model_init : forall s0,
+      H.(h_initial_state) s0 ->
+      ReachableState {| m_actors := initial_actors;
+                        m_state  := s0;
+                     |}
+
+  | model_step : forall (aid : AID) (ms ms' : ModelState) (HIn : In aid (m_actors ms)),
+      is_reachable ms ms' aid HIn ->
+      ReachableState ms ->
+      ReachableState ms'.
+
+  Definition valid_transition (ms : ModelState) (te : TraceElem) (s' : H.(h_state)) :=
+     match te, ms with
+     | trace_elem aid req ret, mkState aa s =>
+       {HIn : In aid aa |
+        let HReq := match find' aid aa HIn with
+                    | a_cont req' _ => req = req'
+                    end in
+        HReq /\ valid_trace_elem te (m_state ms) s'}
+     end.
+
+  Definition apply_trace_elem (ms : ModelState) (te : TraceElem) (s' : H.(h_state))
+             (Hte : valid_transition ms te s') : ModelState.
+    destruct te as [aid req ret].
+    destruct ms as [aa s].
+    destruct Hte as [HIn [Hreq Hs]].
+    destruct (find' aid aa HIn) as [req0 cont].
+    refine (enter_syscall aid req0 cont _ (mkState aa s)).
+    - rewrite <-Hreq.
+      apply (r_return _ _ ret s').
+  Defined.
+
+  Lemma apply_trace_elem_reachable : forall {initial_actors} (ms : ModelState) (te : TraceElem) s',
+      @ReachableState initial_actors ms ->
+      forall Hte : valid_transition ms te s',
+        @ReachableState initial_actors (apply_trace_elem ms te s' Hte).
+  Proof.
+    intros initial_actors ms te s' Hms Hte.
+    destruct te as [aid req ret].
+    destruct ms as [aa s].
+    destruct Hte as [HIn [Hreq Heval]].
+    refine (model_step aid (mkState aa s) _ HIn _ Hms).
+    simpl.
+    destruct (find' aid aa HIn) as [req' cont].
+    destruct Hreq.
+    exists (r_return _ _ ret s').
+    easy.
+  Qed.
+End Actor.
+
+Section ComposeHandlers.
+  Context {AID : Set} `{OrderedType AID}.
+
+  Definition compose_state (h1 h2 : @t AID) : Set :=
+    h_state h1 * h_state h2.
+
+  Definition compose_req (h1 h2 : @t AID) : Set :=
+    h_req h1 + h_req h2.
+
+  Hint Transparent compose_state.
+
+  Definition compose_initial_state (h1 h2 : @t AID) state :=
+    h1.(h_initial_state) (fst state) /\ h2.(h_initial_state) (snd state).
+
+  Hint Transparent compose_initial_state.
+
+  Definition compose_ret_t (h1 h2 : t) (req : compose_req h1 h2) : Set :=
+    match req with
+    | inl l => h1.(h_ret) l
+    | inr r => h2.(h_ret) r
+    end.
+
+  Hint Transparent compose_ret_t.
+
+  Definition ComposeHandlerRet h1 h2 req : Type :=
+    @HandlerRet (compose_req h1 h2)
+                (compose_state h1 h2)
+                req
+                (compose_ret_t h1 h2).
+
+  Definition compose_eval h1 h2
+             (state : compose_state h1 h2)
+             (aid : AID)
+             req
+             (ret : ComposeHandlerRet h1 h2 req) : Prop.
+    refine (
+        (let (s1, s2) := state in
+         match req as req' return (req = req' -> Prop) with
+         | inl req' => fun H => h1.(h_eval) s1 aid req' _
+         | inr req' => fun H => h2.(h_eval) s2 aid req' _
+         end) (eq_refl req));
+      subst;
+      destruct ret;
+      try simpl in reply;
+      constructor; assumption.
+  Defined.
+
+  Definition compose (h1 h2 : t) : t :=
+    {| h_state         := compose_state h1 h2;
+       h_req           := compose_req h1 h2;
+       h_ret           := compose_ret_t h1 h2;
+       h_initial_state := compose_initial_state h1 h2;
+       h_eval          := compose_eval h1 h2;
+    |}.
+End ComposeHandlers.
+
+Global Arguments h_state {_} {_}.
+Global Arguments h_req {_}.
+Global Arguments h_ret {_}.
+Global Arguments h_initial_state {_}.
+Global Arguments h_eval {_}.
+Global Arguments Actor {_} {_}.
+Global Arguments a_cont {_} {_}.
+Global Arguments ModelState {_} {_}.
+Global Arguments m_actors {_} {_} {_}.
+Global Arguments m_state {_} {_} {_}.
+Global Arguments ReachableState {_} {_}.
+Global Arguments model_init {_} {_} {_} {_}.
+Global Arguments PossibleTrace {_} {_}.
 
 Module Mutable.
   Inductive req_t {T : Set} :=
@@ -245,7 +259,7 @@ Module Mutable.
   | put : T -> req_t.
 
   Section defs.
-  Variables (AID T : Set) (initial_state : T -> Prop).
+  Context (AID T : Set) `{AID_ord : OrderedType AID} (initial_state : T -> Prop).
 
   Local Definition ret_t (req : @req_t T) : Set :=
     match req with
@@ -259,7 +273,7 @@ Module Mutable.
     | put x => r_return _ _ I x
     end.
 
-  Definition t : (t AID) :=
+  Definition t : t :=
     {|
       h_state := T;
       h_req := req_t;
@@ -270,7 +284,7 @@ Module Mutable.
 End Mutable.
 
 Module Mutex.
-  Inductive req_t :=
+  Inductive req_t : Set :=
   | grab    : req_t
   | release : req_t.
 
@@ -279,7 +293,7 @@ Module Mutex.
   Section defs.
   Variable AID : Set.
 
-  Local Definition state_t : Type := option AID.
+  Local Definition state_t : Set := option AID.
 
   Local Definition eval_f (s0 : state_t) (aid : AID) (req : req_t) : @HandlerRet req_t state_t req ret_t :=
     match req, s0 with
@@ -288,22 +302,37 @@ Module Mutex.
     | release, _   => r_return _ _ I None
     end.
 
-  Definition t : (t AID) :=
+  Definition t : t :=
     {|
-      h_state := state_t;
-      h_req := req_t;
+      h_state         := state_t;
+      h_req           := req_t;
       h_initial_state := fun s0 => s0 = None;
-      h_eval := fun s0 aid req ret => ret = eval_f s0 aid req;
+      h_eval          := fun s0 aid req ret => ret = eval_f s0 aid req;
     |}.
-  End defs.
 
-  Theorem no_double_grab : forall initial_actors s0
+  Local Notation "aid '@' req '<~' ret" := (@trace_elem AID t aid req ret).
+
+  Theorem no_double_grab : forall (s : state_t) (a1 a2 : AID),
+      ~(@PossibleTrace AID t s
+                      [ a1 @ grab <~ I;
+                        a2 @ grab <~ I
+                      ]).
+  Proof.
+    intros s a1 a2 H.
+    inversion H as [|s' te tt Hvalid Ht]. subst.
+    inversion Ht as [|s'' te' tt' Hvalid' Ht']. subst.
+    simpl in *.
+    destruct s; simpl in *; inversion Hvalid; subst.
+    - easy.
+  Qed.
+  End defs.
 End Mutex.
 
 Module ExampleModelDefn.
   Definition AID : Set := nat.
 
-  Local Definition handler := compose (Mutable.t AID nat (fun a => a = 0)) (Mutex.t AID).
+  Local Definition handler := compose (Mutable.t AID nat (fun a => a = 0))
+                                      (Mutex.t AID).
 
   Notation "'do' V '<-' I ; C" := (@a_cont AID handler (I) (fun V => Some C))
                                     (at level 100, C at next level, V ident, right associativity).
@@ -342,6 +371,4 @@ Module ExampleModelDefn.
     done release.
 
   Local Definition two_actors := add 0 (counter_race 0) (add 1 (counter_race 1) (empty _) : Map [nat, Actor]).
-
-
 End ExampleModelDefn.
